Renamed "ghost method" to "lemma" whenever appropriate (which is most of the time) in the test suite. Removed some assertions that have been rendered unnecessary because of the computations that Dafny instructs the SMT solver to do.

Test/dafny2/Calculations.dfy
@@ -41,12 +41,12 @@ function qreverse(l: List): List
 
 // Here are two lemmas about the List functions.
 
-ghost method Lemma_ConcatNil(xs : List)
+lemma Lemma_ConcatNil(xs : List)
   ensures concat(xs, Nil) == xs;
 {
 }
 
-ghost method Lemma_RevCatCommute(xs : List)
+lemma Lemma_RevCatCommute(xs : List)
   ensures forall ys, zs :: revacc(xs, concat(ys, zs)) == concat(revacc(xs, ys), zs);
 {
 }
@@ -55,7 +55,7 @@ ghost method Lemma_RevCatCommute(xs : List)
 // is given in a calculational style.  The proof is not minimal--some lines can be omitted
 // and Dafny will still fill in the details.
 
-ghost method Theorem_QReverseIsCorrect_Calc(l: List)
+lemma Theorem_QReverseIsCorrect_Calc(l: List)
   ensures qreverse(l) == reverse(l);
 {
   calc {
@@ -69,7 +69,7 @@ ghost method Theorem_QReverseIsCorrect_Calc(l: List)
   }
 }
 
-ghost method Lemma_Revacc_calc(xs: List, ys: List)
+lemma Lemma_Revacc_calc(xs: List, ys: List)
   ensures revacc(xs, ys) == concat(reverse(xs), ys);
 {
   match (xs) {
@@ -93,7 +93,7 @@ ghost method Lemma_Revacc_calc(xs: List, ys: List)
 
 // Here is a version of the same proof, as it was constructed before Dafny's "calc" construct.
 
-ghost method Theorem_QReverseIsCorrect(l: List)
+lemma Theorem_QReverseIsCorrect(l: List)
   ensures qreverse(l) == reverse(l);
 {
   assert qreverse(l)
@@ -105,7 +105,7 @@ ghost method Theorem_QReverseIsCorrect(l: List)
   Lemma_ConcatNil(reverse(l));
 }
 
-ghost method Lemma_Revacc(xs: List, ys: List)
+lemma Lemma_Revacc(xs: List, ys: List)
   ensures revacc(xs, ys) == concat(reverse(xs), ys);
 {
   match (xs) {
@@ -140,7 +140,7 @@ function Fib(n: nat): nat
   if n < 2 then n else Fib(n - 2) + Fib(n - 1)
 }
 
-ghost method Lemma_Fib()
+lemma Lemma_Fib()
   ensures Fib(5) < 6;
 {
   calc {
@@ -160,11 +160,11 @@ ghost method Lemma_Fib()
 /* List length */
 // Here are some proofs that show the use of nested calculations.
 
-ghost method Lemma_Concat_Length(xs: List, ys: List)
+lemma Lemma_Concat_Length(xs: List, ys: List)
   ensures length(concat(xs, ys)) == length(xs) + length(ys);
 {}
 
-ghost method Lemma_Reverse_Length(xs: List)
+lemma Lemma_Reverse_Length(xs: List)
   ensures length(xs) == length(reverse(xs));
 {
   match (xs) {
@@ -193,7 +193,7 @@ ghost method Lemma_Reverse_Length(xs: List)
   }
 }
 
-ghost method Window(xs: List, ys: List)
+lemma Window(xs: List, ys: List)
   ensures length(xs) == length(ys) ==> length(reverse(xs)) == length(reverse(ys));
 {
   calc {
@@ -221,11 +221,11 @@ function ith<a>(xs: List, i: nat): a
   case Cons(x, xrest) => if i == 0 then x else ith(xrest, i - 1)
 }
 
-ghost method lemma_zero_length(xs: List)
+lemma lemma_zero_length(xs: List)
   ensures length(xs) == 0 <==> xs.Nil?;
 {}
 
-ghost method lemma_extensionality(xs: List, ys: List)
+lemma lemma_extensionality(xs: List, ys: List)
   requires length(xs) == length(ys); // (0)
   requires forall i: nat | i < length(xs) :: ith(xs, i) == ith(ys, i); // (1)
   ensures xs == ys;
